Dataflow/Clocking.v
@@ -13,6 +13,9 @@ Inductive clk_var C (x: ident) ck: Prop :=
     PM.find x C = Some ck ->
     clk_var C x ck.
 
+Definition clk_vars C (xs: list ident) ck: Prop :=
+  List.Forall (fun x => clk_var C x ck) xs.
+
 Inductive clk_clock C: clock -> Prop :=
 | CCbase:
     clk_clock C Cbase
@@ -36,6 +39,9 @@ Inductive clk_lexp C: lexp -> clock -> Prop :=
       clk_var C x ck ->
       clk_lexp C (Ewhen e x b) (Con ck x b).
 
+Definition clk_lexps C (les: list lexp)(ck: clock): Prop :=
+  List.Forall (fun le => clk_lexp C le ck) les.
+
 Inductive clk_cexp C: cexp -> clock -> Prop :=
 | Cmerge:
     forall x t f ck,
@@ -55,10 +61,10 @@ Inductive Well_clocked_eq C: equation -> Prop :=
       clk_cexp C ce ck ->
       Well_clocked_eq C (EqDef x (CAexp ck ce))
 | CEqApp:
-    forall x ck f le,
+    forall x ck f les,
       clk_var C x ck ->
-      clk_lexp C le ck ->
-      Well_clocked_eq C (EqApp x f (LAexp ck le))
+      clk_lexps C les ck ->
+      Well_clocked_eq C (EqApp x f (LAexps ck les))
 | CEqFby:
     forall x ck v0 le,
       clk_var C x ck ->
@@ -69,7 +75,7 @@ Inductive Well_clocked_node C: node -> Prop :=
 | SNode:
     forall f i o eqs,
       Forall (Well_clocked_eq C) eqs ->
-      clk_var C i Cbase ->
+      clk_vars C i Cbase ->
       clk_var C o Cbase ->
       Well_clocked_node C (mk_node f i o eqs).
 
@@ -82,8 +88,8 @@ Definition Well_clocked G : Prop :=
 Inductive Has_clock_eq: clock -> equation -> Prop :=
 | HcEqDef: forall x ck ce,
     Has_clock_eq ck (EqDef x (CAexp ck ce))
-| HcEqApp: forall x f ck le,
-    Has_clock_eq ck (EqApp x f (LAexp ck le))
+| HcEqApp: forall x f ck les,
+    Has_clock_eq ck (EqApp x f (LAexps ck les))
 | HcEqFby: forall x v0 ck le,
     Has_clock_eq ck (EqFby x v0 (LAexp ck le)).
 
