Correctness/Proper.v
@@ -117,13 +117,26 @@ Proof.
     destruct sv; simpl; rewrite IH, HMeq; reflexivity.
 Qed.
 
+Instance translate_exps_Proper :
+  Proper (PS.eq ==> eq ==> eq) 
+    (fun M l => List.map (translate_lexp M) l).
+Proof.
+  intros M M' HMeq l.
+  induction l; intros l' Hleq; destruct l'; try discriminate; eauto.
+  injection Hleq; intros.
+  simpl. erewrite IHl; eauto.
+  rewrite HMeq. congruence.
+Qed.
+
 Instance translate_eqn_Proper :
   Proper (PS.eq ==> eq ==> eq) translate_eqn.
 Proof.
   intros M M' HMeq eq eq' Heq; rewrite <- Heq; clear Heq eq'.
+  (* XXX: what is the Proper way to avoid the [rewrite translate_exps_Proper]? *)
   destruct eq as [y e|y f e|y v0 e];
-    (destruct e; simpl; rewrite HMeq; reflexivity).
+    (destruct e; simpl; try (rewrite translate_exps_Proper; eauto); rewrite HMeq; reflexivity).
 Qed.
+
 
 Instance translate_eqns_Proper :
   Proper (PS.eq ==> eq ==> eq) translate_eqns.
